Complete the proof that sf_spec is total! In otherwords, elections satisfying the specification always select some winner. This proof was surprisingly difficult!
Also, some minor progress on the mutual majority criterion proof.
Again, what seems like it should be a straightforward proof is actually
surprisingly difficult.  I think I have now stated the right induction
hypothesis, but the details are fiddly.

src/sf_properties.v
@@ -14,6 +14,75 @@ Section sf_spec_properties.
   Let ballot := list rankSelection.
   Let election := list ballot.
 
+  Check sf_spec.first_choices.
+
+  Lemma next_ranking_elim_unchanged :
+    forall (elim elim':candidate -> Prop) b c r,
+      (forall x, elim x -> elim' x) ->
+      ~elim' c ->
+      sf_spec.next_ranking candidate elim b r ->
+      In c r ->
+      sf_spec.next_ranking candidate elim' b r.
+  Proof.
+    intros.
+    induction H1.
+    * apply sf_spec.next_ranking_eliminated; auto.
+      rewrite Forall_forall in *; firstorder.
+    * apply sf_spec.next_ranking_valid with c; auto.
+  Qed.
+
+  Lemma selected_candidate_elim_unchanged :
+    forall (elim elim':candidate -> Prop) b c,
+      sf_spec.selected_candidate candidate elim b c ->
+      (forall x, elim x -> elim' x) ->
+      ~elim' c ->
+      sf_spec.selected_candidate candidate elim' b c.
+  Proof.
+    intros.
+    destruct H.
+    destruct H2 as [r [Hr Hc]].
+    split.
+    * intro. apply H.
+      destruct H2.
+      elim H2.
+      exists r. eapply next_ranking_elim_unchanged; eauto.
+      destruct H2 as [r' [??]].
+      assert (r = r').
+      { cut (sf_spec.next_ranking candidate elim' b r'); [ apply sf_spec.next_ranking_unique; auto | auto ].
+        eapply next_ranking_elim_unchanged; eauto.
+      }
+      subst r'.
+      right; exists r; split; auto.
+    * exists r; split; auto.
+      eapply next_ranking_elim_unchanged; eauto.      
+  Qed.
+
+  (** As we eliminate candidates, the first-choice counts of the remaining
+      candidates increases monotonically.
+    *)
+  Lemma first_choices_monotone :
+    forall elim elim' e c m n,
+      ~elim' c ->
+      sf_spec.first_choices candidate elim c e m ->
+      sf_spec.first_choices candidate elim' c e n ->
+      (forall x, elim x -> elim' x) ->
+      m <= n.
+  Proof.
+    intros.
+    revert n H1.
+    induction H0; intros.
+    * auto with arith.
+    * inversion H3; subst; clear H3.
+      - cut (n' <= n'0). auto with arith.
+        apply IHfirst_choices; auto.
+      - elim H6.
+        eapply selected_candidate_elim_unchanged; eauto.
+    * inversion H3; subst; clear H3.
+      transitivity n'; auto with arith.
+      apply IHfirst_choices; eauto.
+  Qed.
+
+
   Let sf_may_win_election c e :=
     sf_spec.winner candidate e (fun _ => False) c.
 
@@ -130,84 +199,29 @@ Section sf_spec_properties.
     split; intros.
     destruct (classic (exists c, sf_spec.selected_candidate _ eliminated b c )); auto.
     elim H. clear H.
-    red.
-    destruct (classic (sf_spec.overvote _ eliminated b)); auto.
-    left.
-    red; intros.
-    destruct (classic (eliminated candidate0)); auto.
-    elim H0. clear H0.
-    revert candidate0 rank H1 H2 H3.
-    induction b; intros.
-    elim H1.
-    destruct (classic (exists c, In c a /\ ~eliminated c)).
-    destruct H0 as [c [??]].
-    exists c.
-    split.
-    intro.
-    destruct H5; auto.
-    apply H4.
-    red in H5.
-    apply H5 with a; simpl; auto.
-    exists a; split; simpl; auto.
-    right.
-    split; auto.
-    exists c; split; auto.
-    destruct H1.
-    subst rank.
-    elim H0. eauto.
-    destruct IHb with candidate0 rank; auto.
-    intro. apply H.
-    destruct H4 as [r [??]].
-    exists r. split; simpl; auto.
-    left.
-    split; auto.
+    rewrite sf_spec.exhausted_ballot_next_ranking_iff.
     intros.
-    destruct (classic (eliminated c)); auto.
-    elim H0.
-    eauto.
-    exists x.
-    destruct H4.
-    split; auto.
-    intro.
-    apply H4.
-    destruct H6.
-    left.
-    red; intros.
-    eapply H6.
-    simpl. right; eauto. auto.
-    right.
-    destruct H6 as [r [??]].
-    exists r; split; auto.
-    simpl in H6.
-    destruct H6; auto.
-    destruct H6; auto.
-    destruct H6. subst r.
-    contradiction.
-    destruct H5 as [r [??]].
-    exists r; split ;auto.
-    simpl.
-    left; split; auto.
-    intros.
-    destruct (classic (eliminated c)); auto.
-    elim H0; eauto.
+    destruct (sf_spec.next_ranking_spec candidate eliminated b r); auto.
+    destruct H1 as [c[?[??]]].
+    elim H0. exists c.
+    split; eauto.
+    intro. destruct H4.
+    elim H4. eauto.
+    destruct H4 as [r' [??]].
+    assert (r = r'). { eapply sf_spec.next_ranking_unique; eauto. }
+    subst r'.
+    destruct H5 as [r1 [r2 [?[??]]]].
+    rewrite Forall_forall in H1.
+    apply H7. transitivity c; firstorder.
 
     destruct H as [c ?].
     intros [?|?].
-    assert (~eliminated c).
-    eapply sf_spec.selected_candidate_not_eliminated; eauto.
-    apply H1.
-    destruct H as [r [?[??]]].
-    eapply H0; eauto.
-    clear -H.
-    induction b; simpl in *; intuition.
-    destruct H0 as [x [??]].
-    destruct H as [? [?[??]]].
-    assert( x = x0 ).
-    eapply sf_spec.next_ranking_unique; eauto.
-    subst x0.
+    destruct H as [? [r [??]]].
+    elim H0; eauto.
+    destruct H0 as [r [??]].
+    destruct H.
     apply H.
-    right.
-    exists x. split; auto.
+    right. exists r. split; auto.
   Qed.
 
   Lemma sf_forced_majority (e:election) (eliminated:candidate -> Prop) :
@@ -228,6 +242,7 @@ Section sf_spec_properties.
     subst n. clear H0.
     inversion H2; clear H2; subst.
     inversion H3; clear H3; subst.
+    * 
     destruct n'.
     simpl.
     assert( n = 0 ).
@@ -245,8 +260,7 @@ Section sf_spec_properties.
         exists a. split; simpl; auto.
         destruct H0 as [?[?[??]]].
         exists x; split; auto.
-        clear -H1.
-        induction a; simpl in *; intuition.
+        eapply sf_spec.next_ranking_in_ballot; eauto.
         eapply sf_spec.selected_candidate_not_eliminated; eauto.
         apply IHe; eauto.
         intros. apply H; auto.
@@ -263,7 +277,7 @@ Section sf_spec_properties.
     intros. apply H1; auto.
     destruct H0 as [b [??]].
     exists b; intuition.
-    apply continuing_ballot_selects in H5.
+  * apply continuing_ballot_selects in H5.
     destruct H5 as [c' ?].
     elim H4.
     replace c with c'; auto.
@@ -272,19 +286,30 @@ Section sf_spec_properties.
     destruct H2 as [r [??]].
     exists a. split; simpl; auto.
     exists r; split; simpl; auto.
-    clear -H2.
-    induction a; simpl in *; intuition.
-    eapply sf_spec.selected_candidate_not_eliminated; eauto.
-    inversion H3; clear H3; subst.
+    eapply sf_spec.next_ranking_in_ballot; eauto.
     assert (sf_spec.continuing_ballot _ eliminated a).
     apply continuing_ballot_selects.
     eauto.
-    elim H0; auto.
+    eapply sf_spec.selected_candidate_not_eliminated; eauto.
+  * inversion H3; clear H3; subst.
+    destruct H4. elim H0. auto.
     apply (IHe c winner_votes); auto.
     intros. apply H1; auto.
     destruct H0 as [b [??]].
     exists b; intuition.
   Qed.
+
+    Lemma nonzero_first_choices_selected :
+      forall (eliminated:candidate -> Prop) c e n,
+        sf_spec.first_choices _ eliminated c e n ->
+        n > 0 ->
+        exists b, In b e /\ sf_spec.selected_candidate _ eliminated b c.
+    Proof.
+      intros. induction H.
+      * omega.
+      * simpl; eauto.
+      * destruct IHfirst_choices as [b [??]]; simpl; eauto.
+    Qed.
 
 
   Section sf_spec_existential_induction.
@@ -309,70 +334,110 @@ Section sf_spec_properties.
       (n:nat)
       (viable:list candidate)
       (eliminated:candidate -> Prop),
-      (forall c, In c viable -> exists n, n > 0 /\ sf_spec.first_choices _ eliminated c e n) ->
+       (forall c, In c viable -> sf_spec.participates _ c e) ->
+      (exists c, In c viable /\ exists n, n > 0 /\ sf_spec.first_choices _ eliminated c e n) ->
       (forall c, eliminated c <-> sf_spec.participates _ c e /\ ~In c viable) ->
       1 <= length viable <= n ->
       P eliminated ->
       exists c, Q eliminated c.
     Proof.
       induction n; [ simpl; intros; omega | ].
-      intros.
+      intros viable eliminated Hviable ????.
       destruct (classic (exists c, sf_spec.majority _ eliminated e c)).
       * destruct H3 as [c ?].
         exists c. apply Hbase; auto.
       * destruct (Hind eliminated) as [loser [?[??]]]; auto.
-        + destruct viable. destruct H1. elimtype False. simpl in H1. omega.
-          exists c. apply H. simpl; auto.
+        + destruct H as [c [??]]; eauto.
         + destruct (list_remove_prop candidate viable (eq loser) loser)
             as [viable' [?[??]]]; auto.
           destruct (classic (In loser viable)); auto.
           destruct H4 as [[??]?].
           elim H4. apply H0. split; auto.
           set ( eliminated' := sf_spec.update_eliminated _ eliminated loser).
-          destruct (IHn viable' eliminated') as [c ?]; auto.
-          intros.
-          destruct (H c) as [nc [??]].
-          apply H9; auto.
-admit.           (* first choices monotone with eliminated set *)
-
-          unfold eliminated'.
-          unfold sf_spec.update_eliminated.
-          intuition.
-          apply H0 in H12; intuition.
-          apply H0 in H12; intuition.
-          apply H14. apply H9. auto.
-          subst c.
-          destruct H4 as [[??]?]; auto.
-          subst c; auto.
-          apply H9 in H1.
-          intuition.
-          destruct (classic (c = loser)).
-          subst c. auto.
-          left.
-          apply H0.
-          split; auto.
-          intros. apply H13.
-          apply H8 in H14.
-          intuition.
-          subst. intuition.
-          split; auto.
-          destruct viable'; simpl; auto.
-          - elim H3.
-            exists loser.
-            destruct (H loser) as [nloser [??]]; auto.
-            destruct (classic (In loser viable)); auto.
-            destruct H4 as [[??]?].
-            elim H4. apply H0.
-            split; auto.
-            apply sf_forced_majority with nloser; auto.
+          assert (Hviable' : exists c', In c' viable').
+          { destruct viable'; simpl; auto.
+            destruct H as [c [? [nc [??]]]].
+            exists c.
+            apply H8 in H. destruct H. elim H. subst c.
+            elim H3. exists loser.
+            apply sf_forced_majority with nc; auto.
             intros.
             destruct (H8 c'); auto.
             destruct (classic (In c' viable)); auto.
-            elim H13.
+            elim H12.
             apply H0. split; auto.
-            elim H14.
-          - omega.
-          - omega.
+            elim H13.
+            eauto.
+          }
+          destruct (IHn viable' eliminated') as [c ?]; auto.
+          - intros. apply H9 in H10. intuition.
+          - destruct H as [c [? [cn [??]]]].
+            destruct (classic (c = loser)).
+            subst c.
+            destruct Hviable' as [c' ?].
+            exists c'. split; auto.
+            destruct (sf_spec.sf_first_choices_total candidate eliminated' e c') as [n' ?].
+            destruct (sf_spec.sf_first_choices_total candidate eliminated e c') as [n'' ?].
+            exists n'; split; auto.
+            cut (n'' <= n'). intro Hn''.
+            cut (cn <= n'').  omega.
+            { destruct H4.
+              apply (H15 c'); auto.
+              split.
+              intro. apply H0 in H16. intuition.
+              apply H19.
+              apply H9 in H12; intuition.
+              apply Hviable.
+              apply H9 in H12. intuition.
+            }
+            { apply first_choices_monotone with eliminated eliminated' e c'; auto.
+              intro. hnf in H15. apply H9 in H12.
+              destruct H15.
+              apply H0 in H15.
+              intuition.
+              intuition.
+              intros. hnf. auto.
+            } 
+            
+            exists c; intuition.
+            apply H8 in H. intuition.
+            elim H12; auto.
+            destruct (sf_spec.sf_first_choices_total candidate eliminated' e c) as [cn' ?].
+            exists cn'; split; auto.
+            cut (cn <= cn'). omega.
+            apply first_choices_monotone with eliminated eliminated' e c; auto.
+            intro. hnf in H15.
+            destruct H15.
+            apply H0 in H15.
+            intuition.
+            elim H12; auto.
+            intros. hnf. auto.
+
+          - unfold eliminated'.
+            unfold sf_spec.update_eliminated.
+            intuition.
+            apply H0 in H12; intuition.
+            apply H0 in H12; intuition.
+            apply H14. apply H9. auto.
+            subst c.
+            destruct H4 as [[??]?]; auto.
+            subst c; auto.
+            apply H9 in H1.
+            intuition.
+            destruct (classic (c = loser)).
+            subst c. auto.
+            left.
+            apply H0.
+            split; auto.
+            intros. apply H13.
+            apply H8 in H14.
+            intuition.
+            subst. intuition.
+          - split; auto.
+            destruct viable'; simpl; auto.
+            destruct Hviable' as [?[]].
+            omega.
+            omega.
           - exists c.
             apply H6. auto.
     Qed.
@@ -386,34 +451,46 @@ admit.           (* first choices monotone with eliminated set *)
       destruct (list_remove_prop_weak _ (all_candidates e) eliminated)
                as [viable [?[??]]].
       apply (sf_spec_existential_induction_aux (length viable) viable); auto.
-admit.
-admit.
-admit.
-Qed.
-(*
-      intros.
-      apply H4 in H5.
-
-      intros.
-      split; intros.
-      split.
-      apply H; auto.
-      intro.
-      apply H4 in H6.
-      intuition.
-      destruct H5.
-      apply all_candidates_participates in H5.
-      apply H3 in H5. destruct H5; auto.
-      contradiction.
-      split; auto.
-      destruct H0 as [c0 [??]].
-      destruct (H3 c0).
-      apply all_candidates_participates; auto.
-      destruct viable. elim H6.
-      simpl; auto. omega.
-      contradiction.
+      * intros. apply H4 in H5. destruct H5.
+        apply (all_candidates_participates c e); auto.
+      * destruct H0 as [c [n[??]]].
+        exists c; split; eauto.
+        destruct (nonzero_first_choices_selected eliminated c e n) as [b [??]]; auto.
+        generalize (sf_spec.selected_candidate_not_eliminated _ _ b c H7); intro.
+        assert ( sf_spec.participates candidate c e ).
+        destruct H7.
+        red; exists b. split; auto.
+        destruct H9 as [r [??]].
+        exists r; split; auto.
+        eapply sf_spec.next_ranking_in_ballot; eauto.
+        generalize (all_candidates_participates c e); intros [??].
+        apply H11 in H9.
+        apply H3 in H9.
+        intuition.
+      * intuition.
+        apply H4 in H6. intuition.
+        generalize (all_candidates_participates c e); intros [??].
+        apply H8 in H6.
+        apply H3 in H6.
+        intuition.
+      * intuition.
+        destruct H0 as [c [n [??]]].
+        destruct (nonzero_first_choices_selected eliminated c e n) as [b [??]]; auto.
+        generalize (sf_spec.selected_candidate_not_eliminated _ _ b c H7); intro.
+        assert ( sf_spec.participates candidate c e ).
+        destruct H7.
+        red; exists b. split; auto.
+        destruct H9 as [r [??]].
+        exists r; split; auto.
+        eapply sf_spec.next_ranking_in_ballot; eauto.
+        generalize (all_candidates_participates c e); intros [??].
+        apply H11 in H9.
+        apply H3 in H9.
+        destruct H9.
+        - destruct viable. elim H9.
+          simpl. omega.
+        - contradiction.
     Qed.
-*)
 
   End sf_spec_existential_induction.
 
@@ -465,19 +542,35 @@ Qed.
   Proof.
     intros.
     apply sf_spec_existential_induction with e (fun _ => True); intuition.
-    apply sf_spec.winner_now; auto.
-    destruct (sf_loser_exists e eliminated0) as [loser ?]; auto.
-admit.
-    exists loser; intuition.
-    apply sf_spec.winner_elimination with loser; auto.
+    * apply sf_spec.winner_now; auto.
+    * destruct (sf_loser_exists e eliminated0) as [loser ?]; auto.
+      + destruct H2 as [c [n [??]]].
+        destruct (nonzero_first_choices_selected eliminated0 c e n) as [b [??]]; auto.
+        exists c.
+        generalize (sf_spec.selected_candidate_not_eliminated _ _ b c H6); intro.
+        split; auto.
+        destruct H6.
+        red; exists b. split; auto.
+        destruct H8 as [r [??]].
+        exists r; split; auto.
+        eapply sf_spec.next_ranking_in_ballot; eauto.
+      + exists loser; intuition.
+        apply sf_spec.winner_elimination with loser; auto.
   Qed.
 
+  Definition mutual_majority_invariant (e:election) (group:list candidate) (eliminated:candidate -> Prop) :=
+    majority_satisfies _ 
+      (fun b => prefers_group _ group b /\
+                exists c, In c group /\ ~eliminated c /\
+                          sf_spec.selected_candidate _ eliminated b c)
+      e.
+  
   Theorem sf_mutual_majority :
     mutual_majority_criterion candidate sf_may_win_election.
   Proof.
     red; intros. red.
     cut (forall (eliminated:candidate -> Prop) c,
-           (forall c', eliminated c' -> In c' group -> False) ->
+           mutual_majority_invariant e group eliminated ->
            sf_spec.winner _ e eliminated c ->
            In c group).
     { intuition.
@@ -487,33 +580,145 @@ admit.
       red in H2.
       destruct H as [[cin ?] [cout ?]].
       generalize (H2 cin cout H H4); intros.
-      assert (exists c r, In r b /\ In c r).
-      { clear -H5.
-        induction H5.
-        destruct H.
-        exists cin, r; intuition.
-        simpl; firstorder.
-        firstorder.
+      clear -H2 H3 H5.
+      { induction e; intros.
+      * elim H3.
+      * simpl in H3. destruct H3.
+        + clear IHe. subst b.
+          clear H2.
+          induction H5.
+          - destruct (sf_spec.sf_first_choices_total _ (fun _ => False) ((r::b) :: e) cin) as [n ?].
+            exists cin. exists n. split; auto.
+            inversion H0; subst; clear H0.
+            omega.
+            elim H3; clear H3. split.
+            intro. destruct H0.
+            apply H0.
+            exists r.
+            apply sf_spec.next_ranking_valid with cin; auto.
+            destruct H. auto.
+            destruct H0 as [r' [??]].
+            assert (r = r').
+            eapply sf_spec.next_ranking_unique; eauto.
+            apply sf_spec.next_ranking_valid with cin.
+            destruct H; auto.
+            right; auto.
+            subst r'.
+            destruct H.
+            destruct H1 as [c1 [c2 [?[??]]]].
+            elim H4.
+            transitivity cin; firstorder.
+            exists r. split; auto.
+            apply sf_spec.next_ranking_valid with cin.
+            destruct H; auto.
+            right; auto.
+            destruct H; auto.
+          - destruct IHprefers as [c [n [??]]].
+            exists c. exists n. split; auto.
+            inversion H0; subst; clear H0.
+            apply sf_spec.first_choices_selected.
+            destruct H3. split.
+            intro. apply H0.
+            destruct H2.
+            left. intro.
+            apply H2.
+            destruct H3 as [r ?].
+            exists r. apply sf_spec.next_ranking_eliminated.
+            rewrite Forall_forall. simpl; auto.
+            intros [?[?[??]]]. elim H4.
+            auto.
+            right.
+            destruct H2 as [r [??]].
+            exists r; split; auto.
+            inversion H2; subst; clear H2.
+            auto.
+            destruct H3 as [?[?[??]]]. elim H2.
+            destruct H1 as [r [??]].
+            exists r; split; auto.
+            apply sf_spec.next_ranking_eliminated.
+            rewrite Forall_forall. simpl; auto.
+            intros [?[?[??]]]. elim H3.
+            auto.
+            auto.
+            apply sf_spec.first_choices_not_selected; auto.
+            intro. apply H3.
+            destruct H0. split.
+            intro. apply H0.
+            destruct H2. left.
+            intro. apply H2.
+            destruct H4 as [r ?].
+            exists r.
+            inversion H4; subst; clear H4.
+            auto.
+            elim H9.
+            right.
+            destruct H2 as [r [??]].
+            exists r; split; auto.
+            apply sf_spec.next_ranking_eliminated.
+            rewrite Forall_forall; auto.
+            intros [?[?[??]]]. elim H7.
+            auto.
+            destruct H1 as [r [??]].
+            exists r. split; auto.
+            inversion H1; subst; clear H1.
+            auto.
+            elim H2.
+          - destruct IHprefers as [c [n [??]]].
+            destruct (sf_spec.sf_first_choices_total _ (fun _ => False) ((r::b)::e) c').
+            exists c'. exists x. split; auto.
+            inversion H4; subst; clear H4.
+            omega.
+            elim H8.
+            split.
+            intro. destruct H4.
+            apply H4.
+            exists r.
+            apply sf_spec.next_ranking_valid with c'.
+            destruct H1. auto.
+            auto.
+            destruct H4 as [r' [??]].
+            inversion H4; subst; clear H4.
+            destruct H1.
+            rewrite Forall_forall in H11.
+            apply H11 in H1. auto.
+            destruct H6 as [?[?[?[??]]]].
+            destruct H1.
+            elim H7.
+            transitivity c'; auto.
+            symmetry; auto.
+            exists r; split; auto.
+            2: destruct H1; auto.
+            apply sf_spec.next_ranking_valid with c'.
+            destruct H1; auto.
+            auto.
+
+        + destruct IHe as [c [n [??]]]; auto.
+          destruct (classic (sf_spec.selected_candidate _ (fun _ => False) a c)).
+          exists c. exists (S n).
+          split. omega.
+          apply sf_spec.first_choices_selected; auto.
+          exists c. exists n.
+          split; auto.
+          apply sf_spec.first_choices_not_selected; auto.
       }
-      firstorder.
+      exists x; split; auto.
+      apply (H1 (fun _ => False)); auto.
+      red; simpl; auto.
 admit.
-      exists x. split; auto.
       apply (H1 (fun _ => False)); auto.
-      apply (H1 (fun _ => False)); auto.
+      red; simpl; auto.
+admit.
     }
 
     intros.
     induction H2.
-    red in H0.
-    red in H2.
-    destruct H0 as [n [??]].
+    * red in H0.
+      red in H2.
+      destruct H0 as [n [t [?[??]]]].
+    
  admit. (* a winning candidate is always selected from the group *)
-    apply IHwinner; auto.
-    intros.
-    unfold eliminated' in H5.
-    red in H5.
-    destruct H5.
-    eapply H1; eauto.
-    subst c'.
- admit. (* an eliminated candidate is never selected from the group *)
+
+    * apply IHwinner; auto.
+      hnf.      
+ admit.
   Qed.
